Progress on updating Low* for Blake2 experiment

code/blake2b/experimental/Hacl.Impl.Blake2b.Partial2.fst
@@ -41,9 +41,7 @@ let declassify_word_to_size x =
 (** Define the state *)
 noeq type state_r = {
   hash: hash_wp;
-  prev: p:size128_t{v p <= Spec.Blake2.max_limb Spec.Blake2B};
-  kk: size_t;
-  nblock: size_t;
+  n: size_t;
   pl: l:size_t{v l <= v size_block};
   block: block_p;
 }
@@ -69,11 +67,9 @@ val blake2b_init_partial:
 let blake2b_init_partial state kk k nn =
   blake2b_init state.hash kk k nn;
   [@inline_let]
-  let prev = if kk =. 0ul then 0 else 128 in
+  let n = if kk =. 0ul then 0ul else 1ul in
   { state with
-    prev = to_size128 prev;
-    kk = kk;
-    nblock = 0ul;}
+    n = n; }
 
 
 
@@ -86,36 +82,40 @@ val blake2b_update_partial:
   (requires fun h ->
     state_inv h state /\ live h input /\
     disjoint state.hash input /\ disjoint state.block input /\
-    v state.kk <= 64 /\ (if v state.kk = 0 then v ll < pow2 128 else v ll + 128 < pow2 128))
+    v (state.n *. size_block) + v ll < pow2 128)
   (ensures  fun h0 _ h1 ->
     modifies2 state.hash state.block h0 h1)
 
 let blake2b_update_partial state ll input =
-  (* Compute the remaining space in the partial block *)
-  let rem: r:size_t{v r <= v size_block} = size_block -. state.pl in
-  (* Copy all input or the size available in the partial block *)
-  let ll0 = if ll <=. rem then ll else rem in
-  let input0 = sub input 0ul ll0 in
-  update_sub #MUT #uint8 #size_block state.block state.pl ll0 input0;
-  if not (ll0 =. rem) then state // This needs to be updated
+  let nll = ll /. size_block in
+  if length input = 0 then state else (
+  if not (state.n +. nll +. 2ul <= max_size_t) then state else (
+  let rb = size_block -. state.pl in
+  let ll0 = if ll <. rb then ll else rb in
+  let partial = sub input 0ul ll0 in
+  update_sub #MUT #uint8 #size_block state.block state.pl ll0 partial;
+  if ll <=. rb then ({state with pl = state.pl +. ll0})
   else (
-    blake2b_update_block state.hash (secret state.prev) state.block;
-    (* Handle the remaining blocks *)
-    let ll1 = ll -. ll0 in
-    let input1 = sub input ll0 ll1 in
-    let n = ll1 /. size_block in
-    let ll2 = ll1 %. size_block in
+    let prev = to_u128 (secret ((state.n +. 1ul) *. size_block)) in
+    blake2b_update_block state.hash prev state.block;
+    (* Handle all full blocks available *)
+    let n1 = (ll -. ll0) /. size_block in
+    let input1 = sub input ll0 (ll -. ll0) in
     let h0 = ST.get () in
-    loop_nospec #h0 n state.hash
+
+    loop_nospec #h0 n1 state.hash
     (fun i ->
       let block = sub input1 (i *. size_block) size_block in
       let h1 = ST.get () in
-      blake2b_update_block state.hash (secret state.prev) block);
-    (* Handle the remaining partial block *)
-    let input2 = sub input (ll0 +. ll1) ll2 in
-    update_sub #MUT #uint8 #size_block state.block 0ul ll2 input2;
-    state // This needs to be updated
-  )
+      let prev = to_u128 (secret ((state.n +. i +. 1ul) *. size_block)) in
+      blake2b_update_block state.hash prev block);
+    let state = {state with n = state.n +. n1;} in
+    (* Store the remainder *)
+    let ll2 = (ll -. ll0) %. size_block in
+    let input2 = sub input (ll -. ll2) ll2 in
+    let block = update_sub state.block 0ul ll2 input2 in
+    ({state with pl = ll2;})
+  )))
 
 
 
@@ -133,5 +133,7 @@ val blake2b_finish_partial:
 
 let blake2b_finish_partial nn output state =
   let empty = create 0ul (u8 0) in
-  blake2b_update_last state.hash state.prev 0ul empty;
+  let last = sub state.block 0 state.pl in
+  let prev = to_u128 (state.n *. size_block +. state.pl) in
+  blake2b_update_last state.hash prev state.pl last;
   blake2b_finish nn output state.hash
